tests/fstar/demo/Demo.fst
@@ -13,15 +13,15 @@ let choose
   then let back_'a = fun ret -> Return (ret, y) in Return (x, back_'a)
   else let back_'a = fun ret -> Return (x, ret) in Return (y, back_'a)
 
-(** [demo::mul2_add1]:
+(** [demo::mul3_add1]:
     Source: 'src/demo.rs', lines 13:0-13:31 *)
-let mul2_add1 (x : u32) : result u32 =
-  let* i = u32_add x x in u32_add i 1
+let mul3_add1 (x : u32) : result u32 =
+  let* i = u32_add x x in let* i1 = u32_add i x in u32_add i1 1
 
-(** [demo::use_mul2_add1]:
+(** [demo::use_mul3_add1]:
     Source: 'src/demo.rs', lines 17:0-17:43 *)
-let use_mul2_add1 (x : u32) (y : u32) : result u32 =
-  let* i = mul2_add1 x in u32_add i y
+let use_mul3_add1 (x : u32) (y : u32) : result u32 =
+  let* i = mul3_add1 x in u32_add i y
 
 (** [demo::incr]:
     Source: 'src/demo.rs', lines 21:0-21:31 *)
@@ -52,12 +52,10 @@ let rec list_nth (t : Type0) (n : nat) (l : cList_t t) (i : u32) : result t =
     | CList_CNil -> Fail Failure
     end
 
-(** [demo::list_nth_mut]:
-    Source: 'src/demo.rs', lines 54:0-54:68 *)
-let rec list_nth_mut
-  (t : Type0) (n : nat) (l : cList_t t) (i : u32) :
-  result (t & (t -> result (cList_t t)))
-  =
+(** [demo::list_nth1]: loop 0:
+    Source: 'src/demo.rs', lines 54:0-63:1 *)
+let rec list_nth1_loop
+  (t : Type0) (n : nat) (l : cList_t t) (i : u32) : result t =
   if is_zero n
   then Fail OutOfFuel
   else
@@ -65,99 +63,38 @@ let rec list_nth_mut
     begin match l with
     | CList_CCons x tl ->
       if i = 0
-      then
-        let back_'a = fun ret -> Return (CList_CCons ret tl) in
-        Return (x, back_'a)
-      else
-        let* i1 = u32_sub i 1 in
-        let* (x1, list_nth_mut_back) = list_nth_mut t n1 tl i1 in
-        let back_'a =
-          fun ret ->
-            let* tl1 = list_nth_mut_back ret in Return (CList_CCons x tl1) in
-        Return (x1, back_'a)
+      then Return x
+      else let* i1 = u32_sub i 1 in list_nth1_loop t n1 tl i1
     | CList_CNil -> Fail Failure
     end
 
-(** [demo::list_nth_mut1]: loop 0:
-    Source: 'src/demo.rs', lines 69:0-78:1 *)
-let rec list_nth_mut1_loop
-  (t : Type0) (n : nat) (l : cList_t t) (i : u32) :
-  result (t & (t -> result (cList_t t)))
-  =
-  if is_zero n
-  then Fail OutOfFuel
-  else
-    let n1 = decrease n in
-    begin match l with
-    | CList_CCons x tl ->
-      if i = 0
-      then
-        let back_'a = fun ret -> Return (CList_CCons ret tl) in
-        Return (x, back_'a)
-      else
-        let* i1 = u32_sub i 1 in
-        let* (x1, back_'a) = list_nth_mut1_loop t n1 tl i1 in
-        let back_'a1 =
-          fun ret -> let* tl1 = back_'a ret in Return (CList_CCons x tl1) in
-        Return (x1, back_'a1)
-    | CList_CNil -> Fail Failure
-    end
-
-(** [demo::list_nth_mut1]:
-    Source: 'src/demo.rs', lines 69:0-69:77 *)
-let list_nth_mut1
-  (t : Type0) (n : nat) (l : cList_t t) (i : u32) :
-  result (t & (t -> result (cList_t t)))
-  =
-  list_nth_mut1_loop t n l i
-
-(** [demo::i32_id]:
-    Source: 'src/demo.rs', lines 80:0-80:28 *)
-let rec i32_id (n : nat) (i : i32) : result i32 =
-  if is_zero n
-  then Fail OutOfFuel
-  else
-    let n1 = decrease n in
-    if i = 0
-    then Return 0
-    else let* i1 = i32_sub i 1 in let* i2 = i32_id n1 i1 in i32_add i2 1
-
-(** [demo::list_tail]:
-    Source: 'src/demo.rs', lines 88:0-88:64 *)
-let rec list_tail
-  (t : Type0) (n : nat) (l : cList_t t) :
-  result ((cList_t t) & (cList_t t -> result (cList_t t)))
-  =
-  if is_zero n
-  then Fail OutOfFuel
-  else
-    let n1 = decrease n in
-    begin match l with
-    | CList_CCons x tl ->
-      let* (c, list_tail_back) = list_tail t n1 tl in
-      let back_'a =
-        fun ret -> let* tl1 = list_tail_back ret in Return (CList_CCons x tl1)
-        in
-      Return (c, back_'a)
-    | CList_CNil -> Return (CList_CNil, Return)
-    end
+(** [demo::list_nth1]:
+    Source: 'src/demo.rs', lines 54:0-54:65 *)
+let list_nth1 (t : Type0) (n : nat) (l : cList_t t) (i : u32) : result t =
+  list_nth1_loop t n l i
 
 (** Trait declaration: [demo::Counter]
-    Source: 'src/demo.rs', lines 97:0-97:17 *)
+    Source: 'src/demo.rs', lines 67:0-67:17 *)
 noeq type counter_t (self : Type0) = { incr : self -> result (usize & self); }
 
 (** [demo::{(demo::Counter for usize)}::incr]:
-    Source: 'src/demo.rs', lines 102:4-102:31 *)
+    Source: 'src/demo.rs', lines 72:4-72:31 *)
 let counterUsize_incr (self : usize) : result (usize & usize) =
   let* self1 = usize_add self 1 in Return (self, self1)
 
 (** Trait implementation: [demo::{(demo::Counter for usize)}]
-    Source: 'src/demo.rs', lines 101:0-101:22 *)
+    Source: 'src/demo.rs', lines 71:0-71:22 *)
 let counterUsize : counter_t usize = { incr = counterUsize_incr; }
 
 (** [demo::use_counter]:
-    Source: 'src/demo.rs', lines 109:0-109:59 *)
+    Source: 'src/demo.rs', lines 79:0-79:59 *)
 let use_counter
   (t : Type0) (counterInst : counter_t t) (cnt : t) : result (usize & t) =
-  counterInst.incr cnt
+  let* (_, cnt1) = counterInst.incr cnt in counterInst.incr cnt1
+
+(** [demo::use_vec_index]:
+    Source: 'src/demo.rs', lines 86:0-86:51 *)
+let use_vec_index (i : usize) (v : alloc_vec_Vec u32) : result u32 =
+  alloc_vec_Vec_index u32 usize (core_slice_index_SliceIndexUsizeSliceTInst
+    u32) v i
 
